revised transcript API to use repr

src/tls/HSL.Transcript.fsti
@@ -12,37 +12,45 @@ module HSL.Transcript
 *)
 open FStar.Integers
 open FStar.HyperStack.ST
-
-module G = FStar.Ghost
 module List = FStar.List.Tot
-
 module HS = FStar.HyperStack
 module B = LowStar.Buffer
-
-open Parsers.Handshake13
+module G = FStar.Ghost
 
 module HSM = Parsers.Handshake
 module HSM12 = Parsers.Handshake12
 module HSM13 = Parsers.Handshake13
+
 module PV = Parsers.ProtocolVersion
 module LP = LowParse.Low.Base
-open HSL.Common
 module IncHash = EverCrypt.Hash.Incremental
 
-type bytes = Spec.Hash.Definitions.bytes
+module R = MITLS.Repr
+module R_HS = MITLS.Repr.Handshake
+
+module R_CH = MITLS.Repr.ClientHello
+module CH = Parsers.ClientHello
+
+module R_SH = MITLS.Repr.ServerHello
+module SH = Parsers.ServerHello
+
+type bytes = FStar.Seq.seq uint_8
 
 type alg = Spec.Hash.Definitions.hash_alg
 
+
+let hs_ch = ch:HSM.handshake{HSM.M_client_hello? ch}
+let hs_sh = sh:HSM.handshake{HSM.M_server_hello? sh}
 // assume
-val is_hrr (sh:Parsers.ServerHello.serverHello)
-       : bool
+val is_hrr (sh:hs_sh) : bool
 
 inline_for_extraction
-let hello_retry_request : Type0 = (s: Parsers.ServerHello.serverHello { is_hrr s } )
-//TODO: This does not yet seem to be modeled in Parsers.rfc
+let hello_retry_request : Type0 = 
+  s:hs_sh { is_hrr s }
 
-type retry = Parsers.ClientHello.clientHello
-           & hello_retry_request
+type retry =
+  hs_ch
+  & hello_retry_request
 
 /// `transcript_t`: Transcript for 1.2 and 1.3 have a shared prefix
 /// and then fork to version-specific message types
@@ -64,29 +72,11 @@ let bounded_list 'a n = l:list 'a{List.length l < n}
 let can_extend_bounded_list #a #n (l:bounded_list a n) = List.length l + 1 < n
 
 open Parsers.ClientHello
-let client_hello_has_psk (ch:Parsers.ClientHello.clientHello) =
+let client_hello_has_psk (ch:CH.clientHello) =
   exists (ext:_). 
     List.memP ext ch.extensions /\
     Parsers.ClientHelloExtension.CHE_pre_shared_key? ext /\
     True (* what else do we need? e.g., that it has as many binders as ids? *)
-  
-let client_hello_with_psk =
-  ch:Parsers.ClientHello.clientHello{
-    client_hello_has_psk ch
-  }
-
-let is_truncated_client_hello_bytes (b:bytes) =
-     exists (suffix:bytes).
-      Seq.length b > 0 /\
-      Seq.length suffix > 0 /\
-      (match LP.parse HSM.handshake_parser (b `Seq.append` suffix) with
-       | Some (HSM.M_client_hello ch, _) ->
-         client_hello_has_psk ch
-       | _ -> False)
- 
-let truncated_client_hello_bytes = 
-  b:bytes{ is_truncated_client_hello_bytes b }
-
 
 noeq
 type transcript_t =
@@ -94,24 +84,19 @@ type transcript_t =
            transcript_t
 
   | Hello: retried:option retry ->
-           ch:Parsers.ClientHello.clientHello ->
+           ch:hs_ch ->
            transcript_t
 
-  | Transcript12: ch:Parsers.ClientHello.clientHello ->
-                  sh:Parsers.ServerHello.serverHello -> //Should prescribe the protocol version
+  | Transcript12: ch:hs_ch ->
+                  sh:hs_sh -> //Should prescribe the protocol version
                   rest:bounded_list HSM12.handshake12 max_transcript_size ->
                   transcript_t
 
   | Transcript13: retried:option retry ->
-                  ch:Parsers.ClientHello.clientHello ->
-                  sh:Parsers.ServerHello.serverHello -> //Should prescribe the protocol version
+                  ch:hs_ch ->
+                  sh:hs_sh -> //Should prescribe the protocol version
                   rest:bounded_list HSM13.handshake13 max_transcript_size -> //but requires a dependence on Nego
                   transcript_t
-                  
-  | TruncatedClientHello:
-      retried:option retry ->
-      tch_b:truncated_client_hello_bytes ->
-      transcript_t
       
 let transcript_n (n:nat{n < max_transcript_size}) =
   t:transcript_t{
@@ -120,7 +105,6 @@ let transcript_n (n:nat{n < max_transcript_size}) =
     | Hello _ _ -> True
     | Transcript12 _ _ rest -> List.length rest < n
     | Transcript13 _ _ _ rest -> List.length rest < n
-    | TruncatedClientHello _ _ -> True
   }
 
 /// `transcript_bytes`: The input of the hash algorithm computed by
@@ -133,10 +117,17 @@ let transcript_n (n:nat{n < max_transcript_size}) =
 ///
 /// Note: we want this to be in Tot
 
+// should be at least 
+//   max (handshake12_parser_kind.parser_kind_high,
+//        handshake13_parser_kind.parser_kind_high,
+//        handshake_parser_kind.parser_kind_high)
 unfold // to recover Z3 linearity
-let max_message_size = 16777219 // should be at least max (handshake12_parser_kind.parser_kind_high, handshake13_parser_kind.parser_kind_high, handshake_parser_kind.parser_kind_high)
+let max_message_size = 16777219 
 
-val transcript_bytes (t:transcript_t) : GTot (b: bytes { Seq.length b < max_transcript_size `Prims.op_Multiply` max_message_size })
+val transcript_bytes (t:transcript_t) 
+: GTot (b: bytes { 
+       Seq.length b < max_transcript_size * max_message_size 
+  })
 
 
 /// `state`: Abstract state of the module
@@ -179,10 +170,10 @@ val frame_invariant (#a:_) (s:state a) (t: transcript_t) (h0 h1:HS.mem) (l:B.loc
 ///   -- The transcript's initial state is empty and the hash alg is
 ///      not chosen yet
 val create (r:Mem.rgn) (a:alg)
-  : ST (state a & G.erased transcript_t)
+  : ST (state a & Ghost.erased transcript_t)
        (requires fun _ -> True)
        (ensures fun h0 (s, tx) h1 ->
-         let tx = G.reveal tx in
+         let tx = Ghost.reveal tx in
          tx == Start None /\
          invariant s tx h1 /\
          region_of s == r /\
@@ -194,12 +185,11 @@ unfold
 let extend_hash_pre_common
   #a
   (s:state a)
-  (#rrel #rel: _)
-  (b:LP.slice rrel rel)
+  (#rrel #rel: _) (#b:LP.slice rrel rel) (#x:_) (r:R.repr x b)
   (t:transcript_t)
   (h:HS.mem)
   = invariant s t h /\
-    LP.live_slice h b /\
+    R.valid r h /\
     B.loc_disjoint (B.loc_buffer LP.(b.base)) (footprint s)
 
 unfold
@@ -212,9 +202,9 @@ let extend_hash_post_common
     B.modifies (footprint s) h0 h1
 
 // assume 
-val nego_version (ch:Parsers.ClientHello.clientHello)
-                        (sh:Parsers.ServerHello.serverHello)
-       : Parsers.ProtocolVersion.protocolVersion
+val nego_version (ch:CH.clientHello)
+                 (sh:SH.serverHello)
+       : PV.protocolVersion
 
 let extend_with_hsm 
       (t:transcript_t)
@@ -223,20 +213,24 @@ let extend_with_hsm
 = match t, m with
   | Start retry, HSM.M_client_hello ch ->
     //Missing: consistency between retry and ch
-    Some (Hello retry ch)
+    Some (Hello retry m)
 
   | Hello retry ch, HSM.M_server_hello sh ->
     if None? retry
-    && is_hrr sh
+    && is_hrr m
     then None
     else
       begin
-      match nego_version ch sh, retry with
+      match nego_version 
+             (HSM.M_client_hello?._0 ch)
+             sh,
+            retry
+      with
       | PV.TLS_1p2, None ->
-        Some (Transcript12 ch sh [])
+        Some (Transcript12 ch m [])
 
       | PV.TLS_1p3, _ ->
-        Some (Transcript13 retry ch sh [])
+        Some (Transcript13 retry ch m [])
 
       | _ -> None
       end
@@ -244,326 +238,158 @@ let extend_with_hsm
   | _ ->
     None
 
-let extend_with_tch (t:transcript_t) (tch_b:truncated_client_hello_bytes)
-  : GTot (option transcript_t) =
-  match t with
-  | Start retry ->
-    Some (TruncatedClientHello retry tch_b)
-
-  | _ -> None
-
-let extend_with_binders (t:transcript_t) (binder_b:bytes)
-  : GTot (option transcript_t) =
-  match t with
-  | TruncatedClientHello retry tch_b ->
-    (match LP.parse HSM.handshake_parser (tch_b `Seq.append` binder_b) with
-     | Some (HSM.M_client_hello ch, len) ->
-       if len = Seq.length tch_b + Seq.length binder_b
-       then Some (Hello retry ch)
-       else None
-     | _ -> None)
-  | _ -> None
-
 let extend_with_hsm12 (t:transcript_n (max_transcript_size - 1)) (m:HSM12.handshake12)
   : option transcript_t
-= match t with
-  | Transcript12 ch sh rest ->
-    List.append_length rest [m];
-    Some (Transcript12 ch sh (List.snoc (rest, m)))
-
-  | _ -> None
+  = match t with
+    | Transcript12 ch sh rest ->
+      List.append_length rest [m];
+      Some (Transcript12 ch sh (List.snoc (rest, m)))
+  
+    | _ -> None
 
 
 let extend_with_hsm13 (t:transcript_n (max_transcript_size - 1)) (m:HSM13.handshake13)
   : option transcript_t
-= match t with
-  | Transcript13 retry ch sh rest ->
-    List.append_length rest [m];
-    Some (Transcript13 retry ch sh (List.snoc (rest, m)))
+  = match t with
+    | Transcript13 retry ch sh rest ->
+      List.append_length rest [m];
+      Some (Transcript13 retry ch sh (List.snoc (rest, m)))
+  
+    | _ -> None
 
-  | _ -> None
-
-val extend_tch 
-  (#a:_)
-  (s:state a)
-  (#rrel #rel: _)
-  (b:LowParse.Low.Base.slice rrel rel)
-  (p0:uint_32)
-  (p1:uint_32{p0 < p1})
-  (tx:G.erased transcript_t)
+val extend_hash_hsm
+  (#a:_) (s:state a)
+  (#p #q: _) (#b:LP.slice p q) (r:R_HS.repr b)
+  (tx:G.erased (transcript_n (max_transcript_size - 1)))
   : Stack (G.erased transcript_t)
        (requires fun h ->
          let tx = G.reveal tx in
-         extend_hash_pre_common s b tx h /\
-         Start? tx /\
-         LP.valid HSM.handshake_parser h b p0 /\
-         (let msg = LP.contents HSM.handshake_parser h b p0 in
-          let len = LP.content_length HSM.handshake_parser h b p0 in
-          HSM.M_client_hello? msg /\
-          client_hello_has_psk (HSM.M_client_hello?._0 msg) /\
-          UInt32.v p1 < UInt32.v p0 + len
-       ))
+         extend_hash_pre_common s r tx h /\
+         Some? (extend_with_hsm tx (R.value r)))
        (ensures fun h0 tx' h1 ->
-         let tx = G.reveal tx in
          let tx' = G.reveal tx' in
-         let msg = LP.contents HSM.handshake_parser h0 b p0 in
-         let tch = LP.bytes_of_slice_from_to h0 b p0 p1 in
-         is_truncated_client_hello_bytes tch /\
-         Some? (extend_with_tch tx tch) /\
-         tx' == Some?.v (extend_with_tch tx tch) /\
+         tx' == Some?.v (extend_with_hsm (G.reveal tx) (R.value r)) /\
          extend_hash_post_common s tx' h0 h1)
 
-val extend_tch_binders
-  (#a:_)
-  (s:state a)
-  (#rrel #rel: _)
-  (b:LowParse.Low.Base.slice rrel rel)
-  (p0:uint_32)
-  (p1:uint_32)
-  (p2:uint_32{p0 < p1 /\ p1 < p2})
-  (tx:G.erased transcript_t)
+//TODO: move to a separate module
+let repr_hs12  (#rrel #rel: _) (b:LP.slice rrel rel) =
+  R.repr_p _ b HSM12.handshake12_parser
+
+val extend_hash_hsm12
+  (#a:_) (s:state a)
+  (#p #q: _) (#b:LP.slice p q) (r:repr_hs12 b)
+  (tx:G.erased (transcript_n (max_transcript_size - 1)))
   : Stack (G.erased transcript_t)
-       (requires fun h ->
-         let tx = G.reveal tx in
-         extend_hash_pre_common s b tx h /\
-         TruncatedClientHello? tx /\
-         LP.valid_pos HSM.handshake_parser h b p0 p2 /\
-         (let msg = LP.contents HSM.handshake_parser h b p0 in
-          let tch_b = LP.bytes_of_slice_from_to h b p0 p1 in
-          TruncatedClientHello?.tch_b tx `Seq.equal` tch_b /\
-          HSM.M_client_hello? msg /\
-          client_hello_has_psk (HSM.M_client_hello?._0 msg)
-       ))
-       (ensures fun h0 tx' h1 ->
-         let tx = G.reveal tx in
-         let tx' = G.reveal tx' in
-         let msg = LP.contents HSM.handshake_parser h0 b p0 in
-         let binder_b = LP.bytes_of_slice_from_to h0 b p1 p2 in
-         Some? (extend_with_binders tx binder_b) /\
-         tx' == Some?.v (extend_with_binders tx binder_b) /\
-         extend_hash_post_common s tx' h0 h1)
+    (requires fun h ->
+      let tx = G.reveal tx in
+      extend_hash_pre_common s r tx h /\
+      Some? (extend_with_hsm12 tx (R.value r)))
+    (ensures fun h0 tx' h1 ->
+      let tx = G.reveal tx in
+      let tx' = G.reveal tx' in
+      tx' == Some?.v (extend_with_hsm12 tx (R.value r)) /\
+      extend_hash_post_common s tx' h0 h1)
+
+
+//TODO: move to a separate module
+let repr_hs13  (#rrel #rel: _) (b:LP.slice rrel rel) =
+  R.repr_p _ b HSM13.handshake13_parser
+
+val extend_hash_hsm13
+  (#a:_) (s:state a)
+  (#p #q: _) (#b:LowParse.Low.Base.slice p q) (r:repr_hs13 b)
+  (tx:G.erased (transcript_n (max_transcript_size - 1)))
+  : Stack (G.erased transcript_t)
+    (requires fun h ->
+      let tx = G.reveal tx in
+      extend_hash_pre_common s r tx h /\
+      Some? (extend_with_hsm13 tx (R.value r)))
+    (ensures fun h0 tx' h1 ->
+      let tx = G.reveal tx in       
+      let tx' = G.reveal tx' in
+      tx' == Some?.v (extend_with_hsm13 tx (R.value r)) /\
+      extend_hash_post_common s tx' h0 h1)
+
+val extend_ch_with_psk
+  (#a:_) (s:state a)
+  (#p #q: _) (#b:LowParse.Low.Base.slice p q) (r:R_HS.repr b)
+  (tx:G.erased transcript_t)
+  : StackInline 
+      (Hacl.Hash.Definitions.hash_t a &
+       G.erased transcript_t)
+    (requires fun h ->
+      let tx = G.reveal tx in
+      let hs = R.value r in
+      extend_hash_pre_common s r tx h /\
+      Start? tx /\         
+      HSM.M_client_hello? hs /\
+      client_hello_has_psk (HSM.M_client_hello?._0 hs))
+    (ensures fun h0 (hash, tx') h1 ->
+      let tx = G.reveal tx in
+      let tx' = G.reveal tx' in
+      B.fresh_loc (B.loc_buffer hash) h0 h1 /\
+      B.live h1 hash /\
+      tx' == Hello (Start?.retried tx) (R.value r) /\
+      extend_hash_post_common s tx' h0 h1)
 
 let extend_with_hrr 
        (t:transcript_t)
-       (r:retry) =
-   match t with
-   | Start None -> Some (Start (Some r))
-   | _ -> None
+       (ch:HSM.handshake)
+       (sh:HSM.handshake) =
+  match t, ch, sh with       
+  | Start None, HSM.M_client_hello _, HSM.M_server_hello _ ->
+    if is_hrr sh
+    then Some (Start (Some (ch, sh)))
+    else None
+  | _ ->
+    None
     
 val extend_hrr
-  (#a:_)
-  (s:state a)
-  (#rrel #rel: _)
-  (ch_b:LowParse.Low.Base.slice rrel rel)
-  (p0:uint_32)
-  (p1:uint_32{p0 <= p1})
-  (sh_b:LowParse.Low.Base.slice rrel rel)
-  (q0:uint_32)
-  (q1:uint_32{q0 <= q1})
+  (#a:_) (s:state a)
+  (#p #q:_) (#b:LP.slice p q) (r_ch:R_HS.repr b)
+  (#p' #q':_) (#b':LP.slice p' q') (r_sh:R_HS.repr b')  
   (tx:G.erased transcript_t)
   : Stack (G.erased transcript_t)
       (requires fun h ->
          let tx = G.reveal tx in
-         extend_hash_pre_common s ch_b tx h /\
-         extend_hash_pre_common s sh_b tx h /\         
-         LP.valid_pos HSM.handshake_parser h ch_b p0 p1 /\
-         LP.valid_pos HSM.handshake_parser h sh_b q0 q1 /\         
-         (let ch = LP.contents HSM.handshake_parser h ch_b p0 in
-          let sh = LP.contents HSM.handshake_parser h sh_b q0 in         
-          HSM.M_client_hello? ch /\          
-          HSM.M_server_hello? sh /\                    
-          is_hrr (HSM.M_server_hello?._0 sh) /\
-          Some? (extend_with_hrr tx (HSM.M_client_hello?._0 ch,
-                                     HSM.M_server_hello?._0 sh))))
+         extend_hash_pre_common s r_sh tx h /\
+         Some? (extend_with_hrr tx (R.value r_ch) (R.value r_sh)))
        (ensures fun h0 tx' h1 ->                                     
          let tx = G.reveal tx in
          let tx' = G.reveal tx' in
-         let ch = 
-           HSM.M_client_hello?._0 (LP.contents HSM.handshake_parser h0 ch_b p0)
-         in
-         let sh = 
-           HSM.M_server_hello?._0 (LP.contents HSM.handshake_parser h0 sh_b q0)
-         in         
-         tx' == Some?.v (extend_with_hrr tx (ch, sh)) /\
-         extend_hash_post_common s tx' h0 h1)
+         tx' == Some?.v (extend_with_hrr tx (R.value r_ch) (R.value r_sh)) /\
+         extend_hash_post_common s tx' h0 h1)         
 
-val extend_hash_hsm
-  (#a:_)
-  (s:state a)
-  (#rrel #rel: _)
-  (b:LowParse.Low.Base.slice rrel rel)
-  (p0:uint_32)
-  (p1:uint_32)
-  (tx:G.erased (transcript_n (max_transcript_size - 1)))
-  : Stack (G.erased transcript_t)
-       (requires fun h ->
-         let tx = G.reveal tx in
-         extend_hash_pre_common s b tx h /\
-         LP.valid_pos HSM.handshake_parser h b p0 p1 /\
-         (let msg = LP.contents HSM.handshake_parser h b p0 in
-          Some? (extend_with_hsm tx msg)))
-       (ensures fun h0 tx' h1 ->
-         let tx' = G.reveal tx' in
-         let msg = LP.contents HSM.handshake_parser h0 b p0 in
-         tx' == Some?.v (extend_with_hsm (G.reveal tx) msg) /\
-         extend_hash_post_common s tx' h0 h1)
-
-val extend_hash_hsm12
-  (#a:_)
-  (s:state a)
-  (#rrel #rel: _)
-  (b:LowParse.Low.Base.slice rrel rel)
-  (p0:uint_32)
-  (p1:uint_32)
-  (tx:G.erased (transcript_n (max_transcript_size - 1)))
-  : Stack (G.erased transcript_t)
-       (requires fun h ->
-         let tx = G.reveal tx in
-         extend_hash_pre_common s b tx h /\
-         LP.valid_pos HSM12.handshake12_parser h b p0 p1 /\
-         (let msg = LP.contents HSM12.handshake12_parser h b p0 in
-          Some? (extend_with_hsm12 tx msg)))
-       (ensures fun h0 tx' h1 ->
-         let tx' = G.reveal tx' in
-         let msg = LP.contents HSM12.handshake12_parser h0 b p0 in
-         tx' == Some?.v (extend_with_hsm12 (G.reveal tx) msg) /\
-         extend_hash_post_common s tx' h0 h1)
-
-val extend_hash_hsm13
-  (#a:_)
-  (s:state a)
-  (#rrel #rel: _)
-  (b:LowParse.Low.Base.slice rrel rel)
-  (p0:uint_32)
-  (p1:uint_32)
-  (tx:G.erased (transcript_n (max_transcript_size - 1)))
-  : Stack (G.erased transcript_t)
-       (requires fun h ->
-         let tx = G.reveal tx in
-         extend_hash_pre_common s b tx h /\
-         LP.valid_pos HSM13.handshake13_parser h b p0 p1 /\
-         (let msg = LP.contents HSM13.handshake13_parser h b p0 in
-          Some? (extend_with_hsm13 tx msg)))
-       (ensures fun h0 tx' h1 ->
-         let tx' = G.reveal tx' in
-         let msg = LP.contents HSM13.handshake13_parser h0 b p0 in
-         tx' == Some?.v (extend_with_hsm13 (G.reveal tx) msg) /\
-         extend_hash_post_common s tx' h0 h1)
 
 let max_message_size_lt_max_input_length (a: alg) : Lemma
-  (max_transcript_size `Prims.op_Multiply` max_message_size < Spec.Hash.Definitions.max_input_length a)
+  (max_transcript_size * max_message_size < Spec.Hash.Definitions.max_input_length a)
   [SMTPat (Spec.Hash.Definitions.max_input_length a)] 
  =
-  assert_norm (max_transcript_size `Prims.op_Multiply` max_message_size < pow2 61);
-  assert_norm (max_transcript_size `Prims.op_Multiply` max_message_size < pow2 125)
+  assert_norm (max_transcript_size * max_message_size < pow2 61);
+  assert_norm (max_transcript_size * max_message_size < pow2 125)
 
 val extract_hash
-  (#a:alg)
-  (s:state a)
+  (#a:alg) (s:state a)
   (tag:Hacl.Hash.Definitions.hash_t a)
   (tx:G.erased transcript_t)
   : ST unit
-       (requires (fun h0 ->
-         let tx = G.reveal tx in
-         invariant s tx h0 /\
-         B.live h0 tag /\
-         B.loc_disjoint (footprint s) (B.loc_buffer tag)))
-       (ensures (fun h0 _ h1 ->
-         let open B in
-         let tx = G.reveal tx in
-         invariant s tx h1 /\
-         modifies (loc_union (footprint s) (loc_buffer tag)) h0 h1 /\
-         B.live h1 tag /\
-         B.as_seq h1 tag == Spec.Hash.hash a (transcript_bytes tx)))
+    (requires (fun h0 ->
+      let tx = G.reveal tx in
+      invariant s tx h0 /\
+      B.live h0 tag /\
+      B.loc_disjoint (footprint s) (B.loc_buffer tag)))
+    (ensures (fun h0 _ h1 ->
+      let open B in
+      let tx = G.reveal tx in
+      invariant s tx h1 /\
+      modifies (loc_union (footprint s) (loc_buffer tag)) h0 h1 /\
+      B.live h1 tag /\
+      B.as_seq h1 tag == Spec.Hash.hash a (transcript_bytes tx)))
 
 
 (*
 val free
-
-val extract
-
-
-
-
-let can_extend_with_hsm12 (t:transcript_t) =
-  match t with
-  | Transcript_hello_server _ -> True
-  | Transcript12 _ _ -> True
-  | _ -> False
-
-let can_extend_with_hsm13 (t:transcript_t) =
-  match t with
-  | Transcript_hello_server _ -> True
-  | Transcript13 _ _ -> True
-  | _ -> False
-
-let extend_transcript
-  (t:transcript_t)
-  (msg:HSM.handshake{can_extend_with_hsm t})
-  : GTot transcript_t
-  = match t with
-    | Transcript_nil -> Transcript_hello_server [msg]
-    | Transcript_hello_server msgs -> Transcript_hello_server (msg::msgs)
-
-let extend_transcript12
-  (t:transcript_t)
-  (msg:HSM12.handshake12{can_extend_with_hsm12 t})
-  : GTot transcript_t
-  = match t with
-    | Transcript_hello_server msgs -> Transcript12 msgs [msg]
-    | Transcript12 hmsgs msgs -> Transcript12 hmsgs (msg::msgs)
-
-let extend_transcript13
-  (t:transcript_t)
-  (msg:HSM13.handshake13{can_extend_with_hsm13 t})
-  : GTot transcript_t
-  = match t with
-    | Transcript_hello_server msgs -> Transcript13 msgs [msg]
-    | Transcript13 hmsgs msgs -> Transcript13 hmsgs (msg::msgs)
-
-
-
-// val extend_unhashed_transcript
-//      (s:state)
-//      (#b:LowParse.Low.Base.slice)
-//      (i:irepr b HSM.handshake_parser)
-//   : ST unit
-//     (requires fun h ->
-//       invariant s h /\
-
-
-
-val extend_hash12
-  (s:state)
-  (b:B.buffer uint_8)
-  (p0:uint_32)
-  (p1:uint_32)
-  (msg:G.erased HSM12.handshake12)
-  : ST unit
-       (requires fun h ->
-         extend_hash_pre_common s b h /\
-         can_extend_with_hsm12 (transcript s h) /\
-         valid_parsing12 (G.reveal msg) p0 p1 b h)
-       (ensures (fun h0 _ h1 ->
-         extend_hash_post_common s b h0 h1 /\
-         transcript s h1 == extend_transcript12 (transcript s h0) (G.reveal msg)))
-
-val extend_hash13
-  (s:state)
-  (b:B.buffer uint_8)
-  (p0:uint_32)
-  (p1:uint_32)
-  (msg:G.erased HSM13.handshake13)
-  : ST unit
-       (requires fun h ->
-         extend_hash_pre_common s b h /\
-         can_extend_with_hsm13 (transcript s h) /\
-         valid_parsing13 (G.reveal msg) p0 p1 b h)
-       (ensures (fun h0 _ h1 ->
-         extend_hash_post_common s b h0 h1 /\
-         transcript s h1 == extend_transcript13 (transcript s h0) (G.reveal msg)))
-
-
+*)
 
 (* We need some form of collision resistance adapted to transcripts.
    i.e., if the hashes of two transcripts match then the transcripts
